
\chapter{Details on the Gibbs sampler from section \ref{sec:est_simple}}

\begin{align}
x_{t+1} &= A x_t + R_v v_t \\
\tilde{y}_t &= B x_t + R_w w_t
\end{align}

with $x_1 \sim \mathrm{Normal}(0, \Sigma_1)$ and $v_t \sim \mathrm{Normal}(0, V_t)$ and $w_t \sim \mathrm{Normal}(0, W_t)$

\begin{align}
p(y^Q_{1:T}, \tilde{y}^M_{1:T}, x_{1:T}, \theta) &= \prod_{t=1:T}p_\theta(y^Q_t|x_t) \cdot \prod_{t=1:T}p_\theta(\tilde{y}^M_t|x_t) \cdot p(x_1) \prod_{t=2:T}p_\theta(x_{t+1}|x_t) \cdot p(\theta) \\
p_\theta(\tilde{y}^M_t|x_t) &= p_\theta(\psi^M(L)y^M_t|x_t) = p_\theta(y^M_t|x_t, y^M_{t-(1:q)})
\end{align}

\begin{align}
p(\theta, x_{1:T}|y^Q_{1:T}, y^M_{-q+1:T}) \propto p(y^Q_{1:T}, \tilde{y}^M_{1:T}, x_{1:T}, \theta)
\end{align}

\subsection*{sample from $p(f_{-3:T}|y^Q_{1:T}, \tilde{y}^M_{1:T}, \theta)$}

\section{sample from $p(\psi|f_{-3:T})$}

prior: $p(\phi) \propto 1_{(\phi\text{ is stationary})}$

\begin{align}
\phi &\sim \mathrm{Normal}(\mu_\phi, \Sigma_\phi)\,1_{(\phi\text{ is stationary})} \\
X_\phi &= [f_{0:T-1}, f_{-1:T-2}, \dots f_{1-p:T-p}] \\
y_\phi &= f_{1:T} \\
\mu_\phi &= (X_\phi'X_\phi)^{-1}X_\phi'y_\phi \\
\Sigma_\phi &= \sigma_\epsilon^2 (X_\phi'X_\phi)^{-1}
\end{align}

\section{sample from $p(\mu^M, \lambda^M, {\sigma^2_\eta}^M|\tilde{y}^M_{1:T}, f_{-3:T})$}

\textbf{sample from $p(\mu^M, \lambda^M|\tilde{y}^M_{1:T}, f_{-3:T}, {\sigma^2_\eta}^M)$}\\

\noindent prior: $p(\mu^M, \lambda^M) \propto 1$

\begin{align}
\beta^M = \begin{bmatrix} \mu^M \\ \lambda^M \end{bmatrix} &\sim \mathrm{Normal}\left(\mu_\beta^M, \Sigma_\beta^M \right) \\
X_\beta^M &= [\psi^M(1),\,\psi(L)f_{1:T}] \\
y_\beta^M &= \psi(L)y^M_{1:T} \\
\mu_\beta^M &= (X_\beta'X_\beta)^{-1}X_\beta'y_\beta \\
\Sigma_\beta^M &= {\sigma_\eta^2}^M (X_\beta'X_\beta)^{-1}
\end{align}

\noindent \textbf{sample from $p({\sigma^2_\eta}^M|\tilde{y}^M_{1:T}, f_{-3:T}, \mu^M, \lambda^M)$}\\

\noindent prior: $p({\sigma^2_\eta}^M) \propto ({\sigma^2_\eta}^M)^{-1/2}$

\begin{align}
{\sigma^2_\eta}^M &\sim \mathrm{InvGamma}(a_\eta, b_\eta) \\
u_\eta &=  \tilde{y}^M_{1:T} - \psi^M(1)\mu^M - \lambda^M \psi^M(L)f_t\\
a_\eta &= \frac{T}{2} \\
b_\eta &= \frac{2}{u_\eta'u_\eta}
\end{align}

\section{sample from $p(\psi^M|y^M_{-q+1:T}, \mu^M, \lambda^M, {\sigma^2_\eta}^M)$}

prior: $p(\phi) \propto 1_{(\psi^M\text{ is stationary})}$

\begin{align}
\psi^M &\sim \mathrm{Normal}(\mu_\psi^M, \Sigma_\psi^M) \cdot 1_{(\psi^M\text{ is stationary})}\\
u_{1-i:T-i} &= y^M_{1-i:T-i} - \mu^M - \lambda^M f_{1-i:T-i} \\
X_\psi &= [u_{0:T-1} \dots u_{1-q:T-q}] \\
y_\psi &= u_{1:T} \\
\mu^M_\psi &= {(X_\psi' X_\psi)}^{-1} X_\psi' y_\psi \\ % TODO double superscript
\Sigma^M_\psi &= {\sigma_\eta^2}^M{(X_\psi' X_\psi)}^{-1}
\end{align}

\section{sample from $p(\mu^Q, \lambda^Q, {\sigma^2_\eta}^Q|y^Q_{1:T}, f_{-3:T})$}

\textbf{sample from $p(\mu^Q, \lambda^Q|y^Q_{1:T}, f_{-3:T}, {\sigma^2_\eta}^Q)$}\\

\noindent \textbf{sample from $p({\sigma^2_\eta}^Q|y^Q_{1:T}, f_{-3:T}, \mu^Q, \lambda^Q)$}\\

\section{sample from $p(\psi^Q|y^Q_{1:T}, \mu^Q, \lambda^Q, {\sigma^2_\eta}^Q)$}

prior: $p(\psi^Q) \propto 1_{(\psi^Q\text{ is stationary})}$

\section{Linear regression with variable selection prior}

% TODO there is some stuff missing in the conditioning set

% TODO capital P and p

\begin{align}
\frac{P(\omega_i=1|\cdot)}{P(\omega_i=0|\cdot)} &= \frac{p(y_i|\omega_i=1)}{p(y_i|\omega_i=0)}\cdot \frac{P(\omega_i=1)}{P(\omega_i=0)} \\
&= \frac{p(y_i|\omega_i=1)}{p(y_i|\omega_i=0)}\cdot\frac{\rho}{1-\rho}
\end{align}
\begin{align}
p(y_i|\omega_i=1) &= \int d\lambda_i p(y_i|\lambda_i) p(\lambda_i|\omega_i=1) \\
&\propto \int d\lambda_i \exp{\left(-\frac{1}{2\sigma_i^2}(y_i-\lambda_i f)'(y_i-\lambda_i f)\right)} \exp{\left(-\frac{1}{2\tau^2}\lambda_i^2\right)} \\ 
&\propto \exp{\left(-\frac{y_i'y_i}{2\sigma_i^2} + \frac{\mu_{\lambda_i}^2}{2\sigma_{\lambda_i}^2}\right)} \int d\lambda_i \exp{\left(-\frac{1}{2\sigma_{\lambda_i}^2}(\lambda_i - \mu_{\lambda_i})^2\right)} \\
&\propto \exp{\left(-\frac{y_i'y_i}{2\sigma_i^2} + \frac{\mu_{\lambda_i}^2}{2\sigma_{\lambda_i}^2}\right)} \\
&\propto \exp{\left(-\frac{1}{2}y_i'\left(\frac{1}{\sigma_i^2} - \frac{\sigma_{\lambda_i}^2}{\sigma_i^4} f'f\right)y_i\right)} \\
&\propto \exp{\left(-\frac{y_i'y_i}{2({\tau^2 f'f + \sigma_i^2})}\right)}
\end{align}

where $\sigma_{\lambda_i}^{-2} = \frac{1}{\sigma_i^2}f'f + \frac{1}{\tau^2}$ and $\mu_{\lambda_i} = \sigma_{\lambda_i}^2 \frac{f'y_i}{\sigma_i^2}$

completing the square, integrate out

\begin{align}
p(y_i|\omega_i=1) &= \frac{1}{\sqrt{2\pi(\tau^2 f'f + \sigma^2)}}\exp{\left(-\frac{y_i'y_i}{2\sigma_i^2} + \frac{\mu_{\lambda_i}^2}{2\sigma_{\lambda_i}^2}\right)}
\end{align}

\begin{align}
p(y_i|\omega_i=0) &= \int d\lambda_i\;p(y_i|\lambda_i) p(\lambda_i|\omega_i=0) \\
&= \int d\lambda_i\;p(y_i|\lambda_i) \delta_0(\lambda_i) \\
&= p(y_i|\lambda_i=0) \\
&= \frac{1}{\sqrt{2\pi\sigma^2}}\exp{\left(-\frac{y_i'y_i}{2\sigma^2}\right)}
\end{align}

\begin{align}
\frac{p(y_i|\omega_i=1)}{p(y_i|\omega_i=0)} &= \sqrt{\frac{\sigma^2}{\tau^2 f'f + \sigma^2}}\exp{\left( \frac{\mu_{\lambda_i}^2}{2\sigma_{\lambda_i}^2}\right)} \\
&= \sqrt{\frac{1}{\frac{\tau^2}{\sigma^2} f'f + 1}}\exp{\left( \frac{\mu_{\lambda_i}^2}{2\sigma_{\lambda_i}^2}\right)} \\
&=\sqrt{\frac{\sigma_{\lambda_i}^2}{\tau^2}}\exp{\left( \frac{\mu_{\lambda_i}^2}{2\sigma_{\lambda_i}^2}\right)}
\end{align}

same as the \citet{KaufmannSchumacher2017} result in Appendix A.2

\begin{align}
\frac{p(\lambda_i|\omega_i=1)|_{\lambda_i=0}}{p(\lambda_i|\omega_i=1, \cdot)|_{\lambda_i=0}} 
&= \sqrt{\frac{\sigma_{\lambda_i}^2}{\tau^2}} \exp{\left(-\frac{\lambda_i^2}{2\tau^2}\vert_{\lambda_i=0} + \frac{(\lambda_i-\mu_{\lambda_i})^2}{2\sigma_{\lambda_i}^2}\vert_{\lambda_i=0}\right)} \\
&=\sqrt{\frac{\sigma_{\lambda_i}^2}{\tau^2}}\exp{\left( \frac{\mu_{\lambda_i}^2}{2\sigma_{\lambda_i}^2}\right)}
\end{align}